transformations/Moore2MealyALT/MealyWF.v
@@ -21,7 +21,7 @@ Lemma always_unique_names :
 Qed.
 
 (* fixme : generalise-me *)
-Lemma In_1 : forall (m:Mealy.M) e,
+Lemma In_state : forall (m:Mealy.M) e,
          List.In (StateElement e) (Model.modelElements m) <-> List.In e
     (OptionListUtils.lift_list (get_E_data State_K)
        (Model.modelElements m)).
@@ -40,31 +40,91 @@ Proof.
   }
 Qed.
 
-Lemma in_find : (* fixme : use the concept of discriminant proposition for the proof *)
+Lemma In_transition : forall (m:Mealy.M) e,
+         List.In (TransitionElement e) (Model.modelElements m) <-> List.In e
+    (OptionListUtils.lift_list (get_E_data Transition_K)
+       (Model.modelElements m)).
+Proof.
+  intros m e.
+  split ; intro H.
+  {
+    apply OptionListUtils.In_lift.
+    exists (TransitionElement e). auto.
+  }  
+  {
+    apply OptionListUtils.In_lift in H.
+    destruct H as (e2 & (G & IN2)).
+    destruct e2 ; [ discriminate G | PropUtils.inj G]. 
+    assumption.
+  }
+Qed.
+
+
+Lemma discr  (m : M) : 
+  unique_names m ->
+  forall (i : NodeId),
+    ListUtils.discriminating_predicate
+      (fun x : State_t => NodeId_beq i (State_name x) = true)
+      (OptionListUtils.lift_list (get_E_data State_K)
+         (Model.modelElements m)).
+Proof.
+  intros WF i.
+  unfold ListUtils.discriminating_predicate ; intros.
+  apply WF.
+  apply In_state ; assumption.
+  apply In_state ; assumption.
+  apply internal_NodeId_dec_bl in H1, H2.
+  congruence.
+Qed.
+
+
+Lemma in_find : 
   forall m n e,
     unique_names m ->
     List.In (StateElement e) m.(Model.modelElements) ->
     e.(State_name) = n ->
-    OptionListUtils.find_lift 
-      (get_E_data State_K)
-      (fun s : State_t => (NodeId_beq n s.(State_name))%string)
+    OptionListUtils.find_lift (get_E_data State_K)
+           (fun s : State_t => (NodeId_beq n  s.(State_name))%string)
            m.(Model.modelElements) = 
          Some e.
 Proof.
   intros.
-  rewrite OptionListUtils.find_lift_filter_lift.
-  destruct e ; simpl in * ; subst.
-  match goal with [ |- ?F = _] => destruct F eqn:E ; [ | exfalso ] end.
-  + f_equal. 
-    apply List.find_some in E.
-    destruct E as (IN2 & EQ).
-    apply In_1 in IN2.
-    apply internal_NodeId_dec_bl in EQ. subst. apply H ; auto.
-  + apply List.find_none with (x:= {| State_name := n |}) in E ; [ |  ].
-    simpl in E.
-    rewrite internal_NodeId_dec_lb in E. discriminate. reflexivity.
-     apply In_1.  assumption.
+  eapply OptionListUtils.in_find_lift ; [ | | | exact H0 ].
+  { apply discr. assumption. }
+  { reflexivity. }
+  { apply internal_NodeId_dec_lb. auto. }  
 Qed.
+
+
+
+Lemma getTransition_source_some (s:State_t) t (m:Mealy.M) :
+  unique_names m ->
+  List.In (StateElement s) m.(Model.modelElements) ->
+  State_name s = t.(Transition_source) ->
+  getTransition_source m t = Some s. 
+Proof.
+  intros WF H1 H2.
+  unfold getTransition_source.
+  eapply OptionListUtils.in_find_lift ; [ | | | exact H1 ].
+  { apply discr. assumption. }
+  { reflexivity. }
+  { apply internal_NodeId_dec_lb. auto. }  
+Qed.
+ 
+Lemma getTransition_target_some  (s:State_t) t (m:Mealy.M) :
+  unique_names m ->
+  List.In (StateElement s) m.(Model.modelElements) ->
+  State_name s = t.(Transition_dest) ->
+  getTransition_target m t = Some s. 
+Proof.
+  intros WF H1 H2.
+  unfold getTransition_target.
+  eapply OptionListUtils.in_find_lift ; [ | | | exact H1 ].
+  { apply discr. assumption. }
+  { reflexivity. }
+  { apply internal_NodeId_dec_lb. auto. }  
+Qed.
+
 
 
 (** Each node has only one transition getting out of it for a same input. *)
@@ -76,3 +136,37 @@ Definition determinist (m:Mealy.M) :=
       t1.(Transition_input) = t2.(Transition_input) ->
       t1 = t2.
 
+Lemma truc m :
+  determinist m ->
+  forall s i,
+    ListUtils.discriminating_predicate
+      (fun x : Transition_t =>
+         (i =? Transition_input x)%string = true)
+      (MealySemantics.State_outTransitions m s).
+Proof.
+  intro WF.
+  intros s i.
+  intros t1 t2 H1 H2 P1 P2.
+  unfold State_outTransitions in H1, H2.
+  apply OptionListUtils.filter_lift_in in H1, H2.
+  destruct H1 as ( ? & ? & ? & ?).
+  destruct H2 as ( ? & ? & ? & ?).
+  PropUtils.destruct_match H1 ; [ | discriminate H1].
+  PropUtils.destruct_match H4 ; [ | discriminate H4].
+  destruct x ; [ discriminate H0 | PropUtils.inj H0]. (* monadInv *)
+  destruct x0 ; [ discriminate H3 | PropUtils.inj H3]. (* monadInv *)
+  apply internal_State_t_dec_bl in H1, H4.
+  subst s1 s0.
+  apply WF ; auto ; [ | ].
+  {
+    apply getTransition_source_inv in Heqo, Heqo0.
+    destruct Heqo.
+    destruct Heqo0.
+    congruence.
+  }
+  {
+    apply String.eqb_eq in P1.
+    apply String.eqb_eq in P2.
+    congruence.
+  }
+Qed.
